\subsection {Proofs of convergence}

\subsubsection {Convergence of $\sum_{n=K}^{\infty}{\mathrm{\hat{p}}\left(K \: \middle| \: n,N\right)}$ }
\label{subsubsec:conv1}
\begin{equation}
\mathrm{\hat{p}}\left(K \: \middle| \: n,N\right) = 
\end{equation}
can be transformed to ${b_j}$ which convergence is proved in the next paragraph. (TODO: transformation)

\subsubsection {Convergence of $\sum_{j=0}^{\infty}{b_j}$ }
\label{subsubsec:conv2}

The ratio of coeficients $b_j$ could be expressed as:

\begin{equation}
\frac{b_{j}}{b_{j-1}}\frac{\ln(K+j)}{\ln(K+j-1)}  = \frac{(K+j)}{j}\frac{\ln(K+j)}{\ln(K+j-1)} \frac{\Gamma{((K+j)\alpha^{*})}}{\Gamma{((K+j-1)\alpha^{*}})}\frac{\Gamma{(N+(K+j-1)\alpha^{*})}}{\Gamma({N+(K+j)\alpha^{*})}}.
\end{equation}
Wendel [\ref{Wendel}] proved inequality:
\begin{equation}
\forall \Delta \in \langle0;1\rangle, \forall x > 0: \frac{ \Gamma(x + \Delta)}{\Gamma(x)} \leq x^{\Delta},
\end{equation}
we should realize that $\alpha \in \langle0;1\rangle$ and than see the similarity leading to
\begin{equation}
\frac{b_j}{b_{j-1}} \frac{\ln(K+j)}{\ln(K+j-1)} \leq  \frac{K+j}{j}\frac{\ln(K+j)}{\ln(K+j-1)} {\left( \frac{(K+j-1)\alpha^*}{(K+j-1)\alpha^* + N} \right)}^{\alpha^{*}}
\end{equation}
The Raabe criterion says that series of complex numbers $\sum_{n} a_n$ converges absolutely if $a_n \neq 0$ and there exists $\lim_{n \to \infty} \left( n \left(\frac{|a_n|}{|a_{n+1}|}-1 \right) \right) > 1$

\begin{equation}
\lim_{j \to \infty} j \left( \frac{b_{j-1}}{b_{j}} \frac{\ln(K+j-1)}{\ln(K+j)}   - 1   \right) \geq \lim_{j \to \infty} j \left( \frac{j}{K+j} \frac{\ln(K+j-1)}{\ln(K+j)} {\left( \frac{(K+j-1)\alpha^* + N}{(K+j-1)\alpha^* } \right)}^{\alpha^{*}} - 1   \right) = L.
\end{equation}
Substitution $x:K+j \Leftrightarrow j=x-K$ leads to:
\begin{equation}
\begin{split}
 \lim_{x \to \infty} \left( (x-K)  \left( \frac{x-K}{x} \frac{\ln(x-1)}{\ln(x)} {\left( \frac{(x-1)\alpha^* + N}{(x-1)\alpha^*} \right)}^{\alpha^{*}} - 1   \right) \right) \\ = \lim_{x \to \infty} \left( x  \left( \frac{x-K}{x} \frac{\ln(x-1)}{\ln(x)} {\left( \frac{(x-1)\alpha^* + N}{(x-1)\alpha^*} \right)}^{\alpha^{*}} - 1   \right) \right) \\
= \lim_{x \to \infty}  \left( (x-K) \frac{\ln(x-1)}{\ln(x)} {\left( \frac{(x-1)\alpha^* + N}{(x-1)\alpha^*} \right)}^{\alpha^{*}} - x   \right) = -K + \lim_{x \to \infty}  \left( x \frac{\ln(x-1)}{\ln(x)} {\left( \frac{(x-1)\alpha^* + N}{(x-1)\alpha^*} \right)}^{\alpha^{*}} - x   \right) \\ 
-K + \lim_{x \to \infty}  \left(x {\left( \frac{1+\frac{N-\alpha^{*}}{x\alpha^{*}}}{1-\frac{1}{x}} \right)}^{\alpha^{*}} - x   \right) = -K + \lim_{x \to \infty} \left( x{\left( 1 + \frac{N-\alpha^{*}}{x\alpha^{*}} \right)}^{\alpha^{*}} -x{\left( 1 - \frac{1}{x} \right)}^{\alpha^{*}} \right)
\end{split}
\end{equation}
Substituting $h = \frac{1}{x} \to 0^{+}$:
\begin{equation}
\begin{split}
&= -K + \lim_{h \to 0^{+}} \frac{ \left( 1+\frac{N-\alpha^{*}}{\alpha^{*}}h \right)^{\alpha^{*}} - {(1-h)}^{\alpha^{*}}}{h}  \\ &\stackrel{L'H}{=} -K + \lim_{h \to 0^{+}} \left( {\left( 1+\frac{N-\alpha^{*}}{\alpha^{*}}h \right)}^{\alpha^{*}-1}(N-\alpha^{*}) + \alpha^{*}(1-h)^{\alpha^{*}-1} \right) \\
 &= -K + N - \alpha^{*} + \alpha^{*} \\ 
 L \stackrel{!}{>} 1 & => -K + N > 1 => K \leq N-2
\end{split}
\end{equation}
Thus the series $\sum_{j=0}^{\infty}{b_j}$ absolutely converges when  $K \leq N-2$.

\subsubsection {Convergence of $\sum_{j=0}^{\infty}{b_j \mathrm{ln}(K+j)} $ }
\label{subsubsec:conv3}

\subsubsection {Convergence of $\frac{\sum_{j=0}^{\infty}{b_j \mathrm{ln}(K+j)}}{\sum_{j=0}^{\infty}{b_j}}$ }
\label{subsubsec:conv4}
As both series $\sum_{j=0}^{\infty}{b_j \mathrm{ln}(K+j)}$ and $\sum_{j=0}^{\infty}{b_j}$ converge absolutely, their fraction converges as well.
